src/tls/StreamAE.fst
@@ -8,6 +8,9 @@ open FStar.Heap
 open FStar.HyperHeap
 open FStar.Seq
 open FStar.SeqProperties // for e.g. found
+open FStar.Monotonic.RRef
+open FStar.Monotonic.Seq
+
 open Platform.Error
 open Platform.Bytes
 
@@ -15,17 +18,15 @@ open TLSError
 open TLSConstants
 open TLSInfo
 open StreamPlain
-open MonotoneSeq
-open FStar.Monotonic.RRef
+
 
 let gen parent i = 
   let kv = CoreCrypto.random (CoreCrypto.aeadKeySize (alg i)) in
   let iv = CoreCrypto.random (iv_length i) in
   let writer_r = new_region parent in
-  lemma_repr_bytes_values 0; 
   if authId i then 
     let log : ideal_log writer_r i = alloc_mref_seq writer_r Seq.createEmpty in
-    let ectr: ideal_ctr writer_r i log = MonotoneSeq.new_counter writer_r 0 log in
+    let ectr: ideal_ctr writer_r i log = new_counter writer_r 0 log in
     State #i #Writer #writer_r #writer_r kv iv log ectr
   else 
     let ectr: concrete_ctr writer_r i = m_alloc writer_r 0 in
@@ -34,18 +35,16 @@ let gen parent i =
 
 let genReader parent #i w =
   let reader_r = new_region parent in
-  lemma_repr_bytes_values 0;
   if authId i
   then
     let log : ideal_log w.region i = w.log in
-    let dctr: ideal_ctr reader_r i log = MonotoneSeq.new_counter reader_r 0 log in
+    let dctr: ideal_ctr reader_r i log = new_counter reader_r 0 log in
     State #i #Reader #reader_r #(w.region) w.key w.iv w.log dctr
   else let dctr : concrete_ctr reader_r i = m_alloc reader_r 0 in
     State #i #Reader #reader_r #(w.region) w.key w.iv () dctr
 
 let coerce parent i kv iv =
   let writer_r = new_region parent in
-  lemma_repr_bytes_values 0; 
   let ectr: concrete_ctr writer_r i = m_alloc writer_r 0 in
   State #i #Writer #writer_r #writer_r kv iv () ectr 
 
@@ -61,7 +60,8 @@ let leak #i #role s = State.key s, State.iv s
 //
 // The XORing is a fixed, ad hoc, random permutation; not sure what is gained;
 // we can reason about sequence-number collisions before applying it.
-let aeIV i (seqn:seqn_t) (staticIV:iv i) : lbytes (iv_length i) =
+let aeIV i (seqn:counter) (staticIV:iv i) : lbytes (iv_length i) =
+  lemma_repr_bytes_values seqn;
   let extended = bytes_of_int (iv_length i) seqn in
   xor (iv_length i) extended staticIV
 
@@ -85,7 +85,7 @@ let encrypt #i e l p =
     m_recall ilog;
     let ictr: ideal_ctr e.region i ilog = e.counter in
     testify_counter ictr;
-    MonotoneSeq.write_at_end ilog (Entry l c p); //need to extend the log first, before incrementing the counter for monotonicity; do this only if ideal
+    write_at_end ilog (Entry l c p); //need to extend the log first, before incrementing the counter for monotonicity; do this only if ideal
     m_recall ictr;
     increment_counter ictr;
     m_recall ictr
@@ -94,7 +94,6 @@ let encrypt #i e l p =
     m_write ctr (n + 1);
   c
 
-//val matches: #i:id -> l:plainLen -> c:cipher i l -> entry i -> Tot bool
 
 // decryption, idealized as a lookup of (c,ad) in the log for safe instances
 let decrypt #i d l c =
@@ -102,17 +101,18 @@ let decrypt #i d l c =
   m_recall ctr;
   let j = m_read ctr in
   if authId i 
-  then let ilog = ilog d.log in
-       let log  = m_read ilog in
-       let ictr: ideal_ctr d.region i ilog = d.counter in
-       let _ = testify_counter ictr in //now we know that j <= Seq.length log
-       if j < Seq.length log && matches l c (Seq.index log j) then
-	 begin
-	 increment_counter ictr;
-	 m_recall ctr;
-	 Some (Entry.p (Seq.index log j))
-	 end
-       else None
+  then 
+    let ilog = ilog d.log in
+    let log  = m_read ilog in
+    let ictr: ideal_ctr d.region i ilog = d.counter in
+    let _ = testify_counter ictr in //now we know that j <= Seq.length log
+    if j < Seq.length log && matches l c (Seq.index log j) then
+      begin
+      increment_counter ictr;
+      m_recall ctr;
+      Some (Entry.p (Seq.index log j))
+      end
+    else None
   else //concrete
      let iv = aeIV i j d.iv in
      match CoreCrypto.aead_decrypt (alg i) d.key iv noAD c with
@@ -131,4 +131,3 @@ let decrypt #i d l c =
 - Injective allocation table from i to refs
 
 *)
-
